MCequiv: change m_step and typecheck def to ind; rewrite subst;

Exercises/MCequivScript.sml
@@ -14,7 +14,7 @@ Datatype:
           | Less expr expr | Equal expr expr
           | Divide expr expr | If expr expr expr
           | Apply expr expr
-          | Lam type expr
+          | Lam expr expr
           | Var num
           | Recfun type type (expr -> expr -> expr)
 End
@@ -24,8 +24,8 @@ Datatype:
 	expr =  Lit bool | Equal expr expr
 		  | If expr expr expr
           | Apply expr expr
-          | Lam type expr (* TODO: could change type to expr using typetag *)
-          | Var type num (* TODO: remove type here and add a context that carries the mapping from the variables/numbers to their types *)
+          | Lam expr expr (* TODO maybe remove type (first expr) *)
+          | Var num
           | TypeTag type
 End
 
@@ -45,8 +45,8 @@ Definition isAtom:
 (*	(isAtom (Num _) ⇔ T) ∧ *)
 	(isAtom (Lit _) ⇔ T) ∧
 (*	isAtom (Recfun _ _ _) ∧ *)
-	(isAtom (Var _ _) ⇔ T) ∧
-	(isAtom (Lam _ _ _) ⇔ T) ∧
+	(isAtom (Var _) ⇔ T) ∧
+	(isAtom (Lam _ _) ⇔ T) ∧
 	(isAtom _ ⇔ F)
 End
 
@@ -74,7 +74,7 @@ QED
 
 
 Definition isVar:
-	(isVar (Var _ _) ⇔ T) ∧
+	(isVar (Var _) ⇔ T) ∧
 	(isVar _ ⇔ F)
 End
 
@@ -82,7 +82,7 @@ Theorem non_var_not_isVar[simp]:
 	¬(isVar (Equal e1 e2)) ∧
 	¬(isVar (If e1 e2 e3)) ∧
 	¬(isVar (Apply e1 e2)) ∧
-	¬(isVar (Lam t1 t2 e1)) ∧
+	¬(isVar (Lam t e1)) ∧
 	¬(isVar (Lit b))
 Proof
 	rw[isVar]
@@ -115,19 +115,40 @@ Definition M_step:
 End
 *)
 
+(*
+Definition freevar_cutoff:
+	freevar_cutoff = 10
+End
+*)
+
+
+Definition shift_up_one:
+	shift_up_one e = case e of
+		  Var m => Var (m+1)
+		| _ => e
+End
+
+Definition shift_down_one_bounded:
+	shift_down_one_bounded e = case e of
+		  Var m => if (m > 0) then Var (m-1) else e
+		| _ => e
+End
+
+
 Definition subst:
-(* TODO: use Lit directly *)
-	subst e1 e2 n = if (isVal e1) then e1 else case e1 of
-		Equal a b => Equal (subst a e2 n) (subst b e2 n)
+	subst e1 e2 n = case e1 of
+		Lit b => Lit b
+	  | TypeTag t => TypeTag t
+	  | Equal a b => Equal (subst a e2 n) (subst b e2 n)
 	  | If g a b => If (subst g e2 n) (subst a e2 n) (subst b e2 n)
 	  | Apply a b => Apply (subst a e2 n) (subst b e2 n)
-	  | Lam t1 t2 e => Lam t1 t2 (subst e e2 (n+1))
-	  | Var t m => if (n = m) then e2 else (Var t m)
+	  | Lam t e => Lam t (subst e (shift_up_one e2) (n+1))
+	  | Var m => if (n = m) then e2 else (Var m)
 End
 
 (* (\x (\y. xy)) (Var 0) *)
+(* (\. (\. (Var 1) (Var 0)))) (Var 0) *)
 (* TODO:
-	1. check capture avoiding substitution
 	2. check higher order abstract syntax *)
 
 Definition M_step:
@@ -147,22 +168,20 @@ Definition M_step:
 	M_step (Divide (Num a) b) = Divide (Num a) (M_step b) ∧
 	M_step (Divide a b) = Divide (M_step a) b ∧ *)
 	M_step (Lit e) = Lit e ∧
-	M_step (Var t v) = Var t v ∧
-	M_step (Lam t1 t2 e) = Lam t1 t2 e ∧
+	M_step (Var v) = Var v ∧
+	M_step (Lam t e) = Lam t e ∧
+	M_step (TypeTag t) = (TypeTag t) ∧
 	M_step (Equal (Lit a) (Lit b)) = Lit (a = b) ∧
-(*	M_step (Equal (Lit a) (Lam b)) = Lit False ∧
-	M_step (Equal (Lit a) (Var t b)) = Lit False ∧ *)
 	M_step (Equal (Lit a) b) = Equal (Lit a) (M_step b) ∧
-(*	M_step (Equal (Lam a) (Lit b) = Lit False *)
 	M_step (Equal a b) = Equal (M_step a) b ∧
 	M_step (If (Lit True) t e) = t ∧
 	M_step (If (Lit False) t e) = e ∧
 	M_step (If b t e) = If (M_step b) t e ∧
-	(M_step (Apply (Lam t1 t2 e) e2) =
+	(M_step (Apply (Lam t e) e2) =
 		if isAtom e2 then
-			subst e e2 0
+			shift_down_one_bounded (subst e (shift_up_one e2) 0)
 		else
-			Apply (Lam t1 t2 e) (M_step e2))	∧
+			Apply (Lam t e) (M_step e2))	∧
 	M_step (Apply e1 e2) = Apply (M_step e1) e2
 (*	M_step (Apply rec@(Recfun _ _ f) e2)
 	  | isAtom e2 = f rec e2
@@ -170,6 +189,37 @@ Definition M_step:
 	M_step (Apply e1 e2) = Apply (M_step e1) e2
 *)
 End
+
+
+Inductive M_step_inductive:
+	(∀e. M_step_inductive (Lit e) (Lit e)) ∧
+	(∀v. M_step_inductive (Var v) (Var v)) ∧
+	(∀t e. M_step_inductive (Lam t e) (Lam t e)) ∧
+	(∀t. M_step_inductive (TypeTag t) (TypeTag t)) ∧
+	(∀a b. M_step_inductive (Equal (Lit a) (Lit b)) (Lit (a = b))) ∧
+	(∀a b b'.
+		M_step_inductive b b'
+		⇒ M_step_inductive (Equal (Lit a) b) (Equal (Lit a) b')) ∧
+	(∀a b a'.
+		M_step_inductive a a'
+		⇒ M_step_inductive (Equal a b) (Equal a' b)) ∧
+	(∀t e. M_step_inductive (If (Lit True) t e) t) ∧
+	(∀t e. M_step_inductive (If (Lit False) t e) e) ∧
+	(∀b t e b'.
+		M_step_inductive b b'
+		⇒ M_step_inductive (If b t e) (If b' t e)) ∧
+	(∀t e e2.
+		isAtom e2
+		⇒ M_step_inductive (Apply (Lam t e) e2)
+						   (shift_down_one_bounded (subst e (shift_up_one e2) 0))) ∧
+	(∀t e e2 e2'.
+		M_step_inductive e2 e2'
+		⇒ M_step_inductive (Apply (Lam t e) e2) (Apply (Lam t e) e2')) ∧
+	(∀e1 e2 e1'.
+		M_step_inductive e1 e1'
+		⇒ M_step_inductive (Apply e1 e2) (Apply e1' e2))
+End
+
 
 (* TODO *)
 (*
@@ -187,13 +237,13 @@ Proof
 	Cases_on `e2` >> rw[M_step]
 QED
 
-(* TODO; check isabelle/hol: induct cases gives all theorems like above *)
-
+(*
 Theorem equal_step_size:
 	∀e1 e2. expr_size (M_step (Equal e1 e2)) < expr_size e1 + (expr_size e2 + 1)
 Proof
 	Cases_on `e1` >>
 QED
+*)
 
 (*
 Definition run_M_step:
@@ -216,7 +266,7 @@ End
 (* expr -> SOME type *)
 Definition typeCheck:
 (*	typeCheck (Num n) = IntTy ∧ *)
-	typeCheck (Lit b) = SOME BoolTy ∧
+	(typeCheck Γ (Lit b) = SOME BoolTy) ∧
 (*	typeCheck (Plus e1 e2) = case (typeCheck e1, typeCheck e2) of
 	                           (IntTy, IntTy) -> IntTy
 	                           _ -> error "type error"
@@ -229,39 +279,72 @@ Definition typeCheck:
 	typeCheck (Less e1 e2) = case (typeCheck e1, typeCheck e2) of
 	                           (IntTy, IntTy) -> BoolTy
 	                           _ -> error "type error" *)
-	(typeCheck (Equal e1 e2) = case (typeCheck e1, typeCheck e2) of
+	(typeCheck Γ (Equal e1 e2) = case (typeCheck Γ e1, typeCheck Γ e2) of
 	                        (*   (IntTy, IntTy) -> BoolTy *)
 	                         |  (SOME BoolTy, SOME BoolTy) => SOME BoolTy
 	                         |  _ => NONE (* error "type error" *)) ∧
-	(typeCheck (If c t e) = case (typeCheck c, typeCheck t, typeCheck e) of
+	(typeCheck Γ (If c t e) = case (typeCheck Γ c, typeCheck Γ t, typeCheck Γ e) of
 	   | (SOME BoolTy, tt, te) => if tt = te then tt else NONE (* error "Branches have different types" *)
 	   | _ => NONE (* error "if condition should be bool" *)) ∧
-	(typeCheck (Apply e1 e2) = case (typeCheck e1, typeCheck e2) of
+	(typeCheck Γ (Apply e1 e2) = case (typeCheck Γ e1, typeCheck Γ e2) of
 	   | (SOME (FunTy t1 t2), SOME t1') => if t1 = t1' then (SOME t2)
 	                                  else NONE (* error "Argument doesn't match function" *)
 	   | _ => NONE) ∧ (* error "Can't apply a non-function" *)
-	typeCheck (Lam t1 t2 e) = SOME (FunTy t1 t2) ∧ (* error "Function body doesn't match type signature" *)
-	typeCheck (Var t n) = SOME t ∧
-	typeCheck (TypeTag t) = SOME t
+	(typeCheck Γ (Lam t e) = typeCheck Γ t) ∧ (* error "Function body doesn't match type signature" *)
+	(typeCheck Γ (Var n) = if (n < LENGTH Γ) then (SOME (EL n Γ)) else NONE) ∧
+	(typeCheck Γ (TypeTag t) = SOME t)
 End
 
+(* TODO: change name *)
+Inductive typeCheck_inductive:
+	(∀Γ b. typeCheck_inductive Γ (Lit b) BoolTy) ∧
+	(∀Γ t. typeCheck_inductive Γ (TypeTag t) t) ∧
+	(∀Γ n. (n < LENGTH Γ) ⇒ typeCheck_inductive Γ (Var n) (EL n Γ)) ∧
+	(∀Γ e1 e2.
+	    (typeCheck_inductive Γ e1 BoolTy
+	     ⇒ typeCheck_inductive Γ e2 BoolTy
+		 ⇒ typeCheck_inductive Γ (Equal e1 e2) BoolTy) ∧
+	(∀Γ b t e tt.
+	    typeCheck_inductive Γ b BoolTy
+	    ⇒ typeCheck_inductive Γ t tt
+	    ⇒ typeCheck_inductive Γ e tt
+		⇒ typeCheck_inductive Γ (If b t e) tt) ∧
+	(∀e1 e2 t1 t1' t2 Γ.
+		typeCheck_inductive Γ e1 (FunTy t1 t2)
+		⇒ typeCheck_inductive Γ e2 t1
+		⇒ typeCheck_inductive Γ (Apply e1 e2) t2) ∧
+	(∀e t t1 t2 Γ.
+		typeCheck_inductive Γ t (FunTy t1 t2)
+		⇒ typeCheck_inductive (* TODO: extend Γ and prove e has type t2 *)
+		⇒ typeCheck_inductive Γ (Lam t e) (FunTy t1 t2))
+End
+
+(* Γ, x:t1 |- s:t2 *)
+(* Γ |- \x. s : FunTy t1 t2 *)
 
 Theorem typeCheck_equal_bool_or_none:
-∀e1 e2.	typeCheck (Equal e1 e2) = SOME BoolTy ∨
-		typeCheck (Equal e1 e2) = NONE
+∀Γ e1 e2.	typeCheck Γ (Equal e1 e2) = SOME BoolTy ∨
+			typeCheck Γ (Equal e1 e2) = NONE
 Proof
-	rw[] >> Cases_on `typeCheck e1` >> Cases_on `typeCheck e2` >> gs[typeCheck]
+	rw[] >> Cases_on `typeCheck Γ e1` >> Cases_on `typeCheck Γ e2` >> gs[typeCheck]
 	>> Cases_on `x` >> gs[] >> Cases_on `x'` >> gs[]
 QED
 
 Theorem M_progress:
-	∀e t. typeCheck e = SOME t ⇒ isAtom e ∨ ∃e'. M_step e = e'
+	∀Γ e t. typeCheck Γ e = SOME t ⇒ isAtom e ∨ ∃e'. M_step e = e'
 Proof
 	rw[M_step]
 QED
 
+Theorem M_progress_2:
+	∀Γ e t. typeCheck_inductive Γ e t ⇒ isAtom e ∨ ∃e'. M_step e = e'
+Proof
+	rw[M_step]
+QED
+
+(*
 Theorem M_preservation:
-	∀e e' t. typeCheck e = SOME t ∧ M_step e = e' ⇒ typeCheck e' = SOME t
+	∀Γ e e' t. typeCheck Γ e = SOME t ∧ M_step e = e' ⇒ typeCheck Γ e' = SOME t
 Proof
 	Induct_on `e` >> rw[M_step] >> rw[]
 	>- (Cases_on `e` >> Cases_on `e'` >> rw[M_step]
@@ -290,6 +373,88 @@ Proof
 	        	by metis_tac[typeCheck_equal_bool_or_none] >> fs[])
 		>- ()
 		)
+QED
+*)
+
+Theorem lit_m_step_lit:
+	∀b e. M_step_inductive (Lit b) e ⇒ e = Lit b
+Proof
+	Induct_on `M_step_inductive` >> gs[]
+QED
+
+Theorem typetag_m_step_typetag:
+	∀t e. M_step_inductive (TypeTag t) e ⇒ e = TypeTag t
+Proof
+	Induct_on `M_step_inductive` >> gs[]
+QED
+
+Theorem var_m_step_var:
+	∀n e. M_step_inductive (Var n) e ⇒ e = Var n
+Proof
+	Induct_on `M_step_inductive` >> gs[]
+QED
+
+Theorem lam_m_step_lam:
+	∀t e e'. M_step_inductive (Lam t e) e' ⇒ e' = (Lam t e)
+Proof
+	Induct_on `M_step_inductive` >> gs[]
+QED
+
+Theorem m_step_equal:
+	∀e1 e2 e.
+		M_step_inductive (Equal e1 e2) e
+			⇒ ((∃b. e = Lit b) ∨
+			   (∃e2'. M_step_inductive e2 e2' ∧ e = Equal e1 e2') ∨
+			   (∃e1'. M_step_inductive e1 e1' ∧ e = Equal e1' e2))
+Proof
+	Induct_on `M_step_inductive` >> gs[]
+QED
+
+Theorem m_step_if:
+	∀b t e tt.
+		M_step_inductive (If b t e) tt
+			⇒ ( tt = t ∨
+				tt = e ∨
+			   (∃b'. M_step_inductive b b' ∧ tt = (If b' t e)))
+Proof
+	Induct_on `M_step_inductive` >> gs[]
+QED
+
+Theorem m_step_apply:
+	∀e1 e2 e.
+		M_step_inductive (Apply e1 e2) e
+			⇒ ((isAtom e2 ∧ ∃t le. e1 = Lam t le ∧ e = shift_down_one_bounded (subst le (shift_up_one e2) 0)) ∨
+			   (∃e2'. M_step_inductive e2 e2' ∧ e = Apply e1 e2') ∨
+			   (∃e1'. M_step_inductive e1 e1' ∧ e = Apply e1' e2))
+Proof
+	Induct_on `M_step_inductive` >> gs[]
+QED
+
+Theorem subst_reserves_type:
+	∀Γ e t e2.
+		typeCheck_inductive Γ e t ⇒
+		typeCheck_inductive Γ (subst e (shift_up_one e2) 0) t
+Proof
+	Induct_on `typeCheck_inductive` >> rw[]
+	>- rw[subst, typeCheck_inductive_rules]
+	>- rw[subst, typeCheck_inductive_rules, shift_up_one]
+	>- () metis_tac[subst, shift_up_one]
+QED
+
+Theorem M_preservation_2:
+	∀Γ e e' t. typeCheck_inductive Γ e t ∧ M_step_inductive e e' ⇒ typeCheck_inductive Γ e' t
+Proof
+	Induct_on `typeCheck_inductive` >> rw[M_step_inductive_rules, typeCheck_inductive_rules]
+	>- metis_tac[lit_m_step_lit, typeCheck_inductive_rules]
+	>- metis_tac[typetag_m_step_typetag, typeCheck_inductive_rules]
+	>- metis_tac[var_m_step_var, typeCheck_inductive_rules]
+	>- (drule m_step_equal >> metis_tac[typeCheck_inductive_rules])
+	>- (drule m_step_if >> metis_tac[typeCheck_inductive_rules])
+	>- (rename[`M_step_inductive (Apply e1 e2) e`] >>
+		drule m_step_apply >> rw[]
+		>- ()
+		>> metis_tac[typeCheck_inductive_rules])
+	>> metis_tac[lam_m_step_lam, typeCheck_inductive_rules]
 QED
 
 (*
